#+AUTHOR: EXr0n
#+TITLE: Derivative Rules
* Basics
** Monomial
   $$\frac{\partial}{\partial x} x^a = ax^{a-1}$$
** Exponential
   $$\frac{\partial}{\partial x} a^x = \left(\ln a\right)a^x$$
* Composing
** Sum
   $$\frac{\partial}{\partial x} (f+g)(x) = \frac{\partial}{\partial x}f(x) + \frac{\partial}{\partial x}g(x)$$
** Product
   $$\frac{\partial}{\partial x} (fg)(x) = \left(f\frac{\partial}{\partial x}g\right)(x) + \left(g\frac{\partial}{\partial x}f\right)(x)$$
** Product
   $$\frac{\partial}{\partial x} \left(\frac{f}{g}\right)(x) = \frac{\left(g\frac{\partial}{\partial x}f\right)(x) - \left(f\frac{\partial}{\partial x}g\right)(x)}{g^2(x)}$$
