#+TITLE: Handout 17 Riemann Sums Additional Exercises
#+AUTHOR: Exr0n
* Exercises
** interpreting in terms of area
   [[file:./KBe21math401srcHandout17AdditionalExercises.jpg]]

#+begin_export latex
\setcounter{subsection}{2}
#+end_export

** subtracting integrals
   I expect
   \[\begin{aligned}
   \int_1^2f(x)dx = \int_1^5f(x)dx - \int_2^5f(x)dx = -3-4 = -7
   \end{aligned}\]

   In fact, I expect
   \[\begin{aligned}
   \int_a^bf(x)dx + \int_b^cf(x)dx = \int_a^cf(x)dx
   \end{aligned}\]
** show $\int_a^b x^2dx = \frac{b^3-a^3}{3}$
   (see attached pages)


   Keep in mind
   \[\begin{aligned}
   \sum_{k=1}^n af(x) = a\sum_{k=1}^n f(x)\\
   \sum_{k=1}^n \left( a+f(x)\right)  = an + \sum_{k=1}^{n} f(x)
   \end{aligned}\]


   \[\begin{aligned}
   \int_a^b x^2 dx &= \lim_{n\to \infty} \sum_{k=1}^n \left( \frac{b-a}{n} \left( a+k\frac{b-a}{n}\right) ^2\right)\\
   &= \lim_{n\to \infty} \frac{b-a}{n} \sum_{k=1}^n \left( a+k\frac{b-a}{n}\right) ^2\\
   &= \lim_{n\to \infty} \frac{b-a}{n} \sum_{k=1}^n \left( a^2+\left( k\frac{b-a}{n}\right) ^2 + 2ak\frac{b-a}{n}\right) \\
   &= \lim_{n\to \infty} \frac{b-a}{n} \sum_{k=1}^n a^2+\sum_{k=1}^n \left( k\frac{b-a}{n}\right) ^2 +\sum_{k=1}^n  2ak\frac{b-a}{n} \\
   &= \lim_{n\to \infty} \frac{b-a}{n} \left( a^2n +\sum_{k=1}^n k^2\left(\frac{b-a}{n}\right)^2 +2a\frac{b-a}{n}\sum_{k=1}^n k\right)  \\
   &= \lim_{n\to \infty} \frac{b-a}{n} \left( a^2n + \left(\frac{b-a}{n}\right)^2\sum_{k=1}^n k^2 +2a\frac{b-a}{n}\sum_{k=1}^n k\right)  \\
   &= \lim_{n\to \infty} \frac{b-a}{n} \left( a^2n + \left(\frac{b-a}{n}\right)^2 \frac{n(n+1)(2n+1)}{6} +2a\frac{b-a}{n}\frac{n(n+1)}{2}\right)  \\
   &= \lim_{n\to \infty} (b-a) \left( a^2 + \left(\frac{b-a}{n}\right)^2 \frac{(n+1)(2n+1)}{6} +\cancel{2}a\frac{b-a}{n}\frac{(n+1)}{\cancel{2}}\right)  \\
   &= \lim_{n\to \infty} (b-a) \left( a^2 + \frac{(b-a)^2}{n^2} \left( n\frac{(2n+1)}{6} + \frac{(2n+1)}{6}\right) +a\frac{b-a}{n}(n+1)\right)  \\
   &= \lim_{n\to \infty} (b-a) \left( a^2 + \frac{(b-a)^2}{n^2} \left( n\frac{(2n+1)}{6} + \frac{(2n+1)}{6}\right) +a\cancel{n}\frac{b-a}{\cancel{n}}+a\frac{b-a}{n}\right)  \\
   &= \lim_{n\to \infty} (b-a) \left( a^2 + \frac{(b-a)^2}{n^2} \left( n\frac{(2n+1)}{6} + \frac{(2n+1)}{6}\right) +a(b-a) +\cancelto{0}{a\frac{b-a}{n}}\right)  \\
   &= \lim_{n\to \infty} (b-a) \left( a^2 + \frac{(b-a)^2}{n^{\cancel{2}} } \cancel{n} \frac{(2n+1)}{6} + \cancelto{0}{\frac{(b-a)^2}{n^2} \frac{(2n+1)}{6}} +a(b-a) \right)  \\
   &= \lim_{n\to \infty} (b-a) \left( a^2 + \frac{(b-a)^2}{n} \frac{(2n+1)}{6} + a(b-a) \right)  \\
   &= \lim_{n\to \infty} (b-a) \left( a^2 + \frac{(b-a)^2}{n} \frac{(2n+1)}{6} + a(b-a) \right)  \\
   \end{aligned}\]
