#+TITLE: Handout 20: u-substitution
* $\int \frac{\sqrt{x-1}}{x} dx$

  Let $u= \sqrt{x-1}$, $du = \frac{1}{2\sqrt{x-1}}$
  \[\begin{aligned}
  \int \frac{\sqrt{x-1}}{x} dx &= \int \frac{u}{TODO} dx
  \end{aligned}\]

* 2
* 3
* 4
* 5
* $\int \tan^2x +1 dx$

  \[\begin{aligned}
  \int \tan^2x +1 dx &= \int \sec^2x -1 +1 dx \\
  &= \int \sec^2x dx \\
  \text{Let} u = x, du = 1\\
  &= \int \sec^2u du \\
  &= \tan u +C\\
  &= \boxed{\tan x +C}
  \end{aligned}\]

* 7

* 8

* $\int \frac{\sec ^2 x}{\csc x} sin x dx$

  \[\begin{aligned}
  \int \frac{\sec ^2 x}{\csc x} sin x dx &= \int \tan^2 x dx \\
  &= \int \sec^2x - 1 dx\\
  &= \int \sec^2 x dx - \int 1 dx \\
  &= \tan x - x
  \end{aligned}\]

* 10

* $\int \frac{e^{2 \ln \sin x}+e^{2\ln \cos x}}{e^{2 \ln \tan x} + e^{2 \ln 1}} dx$


  \[\begin{aligned}
  \int \frac{e^{2 \ln \sin x}+e^{2\ln \cos x}}{e^{2 \ln \tan x} + e^{2 \ln 1}} dx &= \int \frac{\sin^2 x + \cos ^2 x}{tan^2x + 1} dx
  \end{aligned}\]


* 12

* 13

* 14
