#+TITLE: Algebra with Integrals
* additive

  \[\begin{aligned}

  \end{aligned}\]

* change of lower bound
  \[\begin{aligned}
  \int_{a}^{b} f(x) dx + \int_{b}^{c} f(x) dx = \int_{a}^{c} f(x) dx\\
  \implies \int_{a}^{x} f(t) dt = \int_{b}^{x} f(t) dt - \int_{a}^{b} f(t) dt
  \end{aligned}\]

* [[file:KBrefFundamentalTheoremOfCalculus.org][fundamental theorem of calculus]]

  \[\begin{aligned}
  \int_{}^{} f'(x) dx = f(x) + C\\
  \frac{d}{dx} \int_{}^{} f(x) dx = f(x)\\
  \frac{d}{dx} \int_{a}^{x} f(t) dt = f(x)
  \end{aligned}\]

  (second one doesn't have a $+C$ because the derivative sends that to zero)
